<?xml version="1.0"?>
<rdf:RDF
    xmlns:rdf="http://www.w3.org/1999/02/22-rdf-syntax-ns#"
    xmlns="http://discovery-project.eu/ontologies/scholar/0.1/"
    xmlns:protege="http://protege.stanford.edu/plugins/owl/protege#"
    xmlns:foaf="http://xmlns.com/foaf/0.1/"
    xmlns:xsp="http://www.owl-ontologies.com/2005/08/07/xsp.owl#"
    xmlns:owl="http://www.w3.org/2002/07/owl#"
    xmlns:xsd="http://www.w3.org/2001/XMLSchema#"
    xmlns:swrl="http://www.w3.org/2003/11/swrl#"
    xmlns:swrlb="http://www.w3.org/2003/11/swrlb#"
    xmlns:rdfs="http://www.w3.org/2000/01/rdf-schema#"
  xml:base="http://discovery-project.eu/ontologies/scholar/0.1/">
  <owl:Ontology rdf:about=""/>
  <rdfs:Class rdf:about="http://discovery-project.eu/ontologies/scholar/0.1/Event">
    <rdfs:label xml:lang="en">Event</rdfs:label>
    <rdfs:comment xml:lang="en">An Event is something that happens at a certain point in time. Examples can be the French Revolution, the election of a US president and so on. Note that in some cases an Event can be considered also a Concept in certain contexts (e.g. the French Revolution). In these cases such an instance can belong to the two classes at the same time.</rdfs:comment>
    <rdfs:subClassOf>
      <rdfs:Class rdf:about="http://discovery-project.eu/ontologies/scholar/0.1/Subject"/>
    </rdfs:subClassOf>
  </rdfs:Class>
  <rdfs:Class rdf:about="http://discovery-project.eu/ontologies/scholar/0.1/FictionalEntity">
    <rdfs:subClassOf>
      <rdfs:Class rdf:about="http://discovery-project.eu/ontologies/scholar/0.1/Subject"/>
    </rdfs:subClassOf>
    <rdfs:label xml:lang="en">Fictional Entity</rdfs:label>
    <rdfs:comment xml:lang="en">A Fictional Entity is something that exists within a story, a literary work or a artwork in general. It can be a character of a movie (e.g. Batman), a place (e.g. Gotham City), a phisical object (e.g. the Bat-Mobile), etc. In these cases an instance of this class can be at the same time an instance of other classes.</rdfs:comment>
  </rdfs:Class>
  <rdfs:Class rdf:about="http://discovery-project.eu/ontologies/scholar/0.1/Concept">
    <rdfs:comment xml:lang="en">A Concept is a topic, often an abstract, non physical entity that a Source can refer to..</rdfs:comment>
    <rdfs:label xml:lang="en">Concept</rdfs:label>
    <rdfs:subClassOf>
      <rdfs:Class rdf:about="http://discovery-project.eu/ontologies/scholar/0.1/Subject"/>
    </rdfs:subClassOf>
  </rdfs:Class>
  <rdfs:Class rdf:about="http://discovery-project.eu/ontologies/scholar/0.1/PrimarySource">
    <rdfs:comment xml:lang="en">An artifact that is considered a primary material in a given domain (e.g. referrign to a specific author or philosophical movement).</rdfs:comment>
    <rdfs:subClassOf>
      <rdfs:Class rdf:about="http://discovery-project.eu/ontologies/scholar/0.1/Source"/>
    </rdfs:subClassOf>
    <rdfs:label xml:lang="en">Primary Source</rdfs:label>
  </rdfs:Class>
  <rdfs:Class rdf:about="http://discovery-project.eu/ontologies/scholar/0.1/Subject">
    <rdfs:label xml:lang="en">Subject</rdfs:label>
    <rdfs:comment xml:lang="en">A Subject is an entity that can be mentioned within a Source. For example a person can be the subject of a picture, a character can be the subject of a story. Subclasses of this class represent more specific types of subjects.</rdfs:comment>
  </rdfs:Class>
  <rdfs:Class rdf:about="http://discovery-project.eu/ontologies/scholar/0.1/Place">
    <rdfs:label xml:lang="en">Place</rdfs:label>
    <rdfs:subClassOf rdf:resource="http://discovery-project.eu/ontologies/scholar/0.1/Subject"/>
    <rdfs:comment xml:lang="en">A Place is something that has a precise and fixed geographical position. For example a city or a building.</rdfs:comment>
  </rdfs:Class>
  <rdfs:Class rdf:about="http://discovery-project.eu/ontologies/scholar/0.1/Person">
    <rdfs:comment xml:lang="en">A Person is a human being.</rdfs:comment>
    <rdfs:subClassOf rdf:resource="http://discovery-project.eu/ontologies/scholar/0.1/Subject"/>
    <rdfs:label xml:lang="en">Person</rdfs:label>
  </rdfs:Class>
  <rdfs:Class rdf:about="http://discovery-project.eu/ontologies/scholar/0.1/PhysicalObject">
    <rdfs:subClassOf rdf:resource="http://discovery-project.eu/ontologies/scholar/0.1/Subject"/>
    <rdfs:label xml:lang="en">Object</rdfs:label>
    <rdfs:comment xml:lang="en">A Physical Object is a material, concrete thing. For example a guitar or a painting.</rdfs:comment>
  </rdfs:Class>
  <rdfs:Class rdf:about="http://discovery-project.eu/ontologies/scholar/0.1/SecondarySource">
    <rdfs:label xml:lang="en">Secondary Source</rdfs:label>
    <rdfs:comment xml:lang="en">An artifact that is considered a secondary material in a given domain (e.g. a commentary of a primary source wrote by a scholar).</rdfs:comment>
    <rdfs:subClassOf>
      <rdfs:Class rdf:about="http://discovery-project.eu/ontologies/scholar/0.1/Source"/>
    </rdfs:subClassOf>
  </rdfs:Class>
  <rdfs:Class rdf:about="http://discovery-project.eu/ontologies/scholar/0.1/Source">
    <rdfs:comment xml:lang="en">A Source is an artifact or document that is matter of study. It can be the digital representation of a real world artifact as well as a natively electronic document (e.g. a web page, a picture).</rdfs:comment>
    <rdfs:label xml:lang="en">Source</rdfs:label>
  </rdfs:Class>
  <owl:ObjectProperty rdf:about="http://discovery-project.eu/ontologies/scholar/0.1/isAuthorOf">
    <owl:inverseOf>
      <owl:ObjectProperty rdf:about="http://discovery-project.eu/ontologies/scholar/0.1/hasAuthor"/>
    </owl:inverseOf>
    <rdfs:comment xml:lang="en">The author of a Source is the human being (Person) who produced it.</rdfs:comment>
    <rdfs:domain rdf:resource="http://discovery-project.eu/ontologies/scholar/0.1/Person"/>
    <rdfs:label xml:lang="en">is author of</rdfs:label>
    <rdfs:range rdf:resource="http://discovery-project.eu/ontologies/scholar/0.1/Source"/>
  </owl:ObjectProperty>
  <owl:ObjectProperty rdf:about="http://discovery-project.eu/ontologies/scholar/0.1/isPartOf">
    <rdfs:comment xml:lang="en">This relation of the inverse of the 'has Part' relation. It specifies that a Source is composed by an other Source. For example a page is a part of the entire book.</rdfs:comment>
    <rdfs:range rdf:resource="http://discovery-project.eu/ontologies/scholar/0.1/Source"/>
    <rdfs:domain rdf:resource="http://discovery-project.eu/ontologies/scholar/0.1/Source"/>
    <rdfs:label xml:lang="en">is part of</rdfs:label>
    <owl:inverseOf>
      <owl:ObjectProperty rdf:about="http://discovery-project.eu/ontologies/scholar/0.1/hasPart"/>
    </owl:inverseOf>
  </owl:ObjectProperty>
  <owl:ObjectProperty rdf:about="http://discovery-project.eu/ontologies/scholar/0.1/isCommentedBy">
    <rdfs:label xml:lang="en">is commented by</rdfs:label>
    <rdfs:subPropertyOf>
      <owl:ObjectProperty rdf:about="http://discovery-project.eu/ontologies/scholar/0.1/isSubjectOf"/>
    </rdfs:subPropertyOf>
    <rdfs:domain rdf:resource="http://discovery-project.eu/ontologies/scholar/0.1/Subject"/>
    <rdfs:range rdf:resource="http://discovery-project.eu/ontologies/scholar/0.1/Source"/>
    <rdfs:comment xml:lang="en">This relation is the inerse of the 'comments' relation. It specifies that a Subject is defined by a given Source.</rdfs:comment>
    <owl:inverseOf>
      <owl:ObjectProperty rdf:about="http://discovery-project.eu/ontologies/scholar/0.1/comments"/>
    </owl:inverseOf>
  </owl:ObjectProperty>
  <owl:ObjectProperty rdf:about="http://discovery-project.eu/ontologies/scholar/0.1/comments">
    <rdfs:subPropertyOf>
      <owl:ObjectProperty rdf:about="http://discovery-project.eu/ontologies/scholar/0.1/hasSubject"/>
    </rdfs:subPropertyOf>
    <rdfs:label xml:lang="en">comments</rdfs:label>
    <rdfs:domain rdf:resource="http://discovery-project.eu/ontologies/scholar/0.1/Source"/>
    <rdfs:comment xml:lang="en">This relation specifies that a Source comments (expresses an opinion) on a Subject.</rdfs:comment>
    <rdfs:range rdf:resource="http://discovery-project.eu/ontologies/scholar/0.1/Subject"/>
    <owl:inverseOf rdf:resource="http://discovery-project.eu/ontologies/scholar/0.1/isCommentedBy"/>
  </owl:ObjectProperty>
  <owl:ObjectProperty rdf:about="http://discovery-project.eu/ontologies/scholar/0.1/isSubjectOf">
    <rdfs:range rdf:resource="http://discovery-project.eu/ontologies/scholar/0.1/Source"/>
    <rdfs:label xml:lang="en">is subject of</rdfs:label>
    <owl:inverseOf>
      <owl:ObjectProperty rdf:about="http://discovery-project.eu/ontologies/scholar/0.1/hasSubject"/>
    </owl:inverseOf>
    <rdfs:comment xml:lang="en">This relation is the inverse of the 'has subject' relation. It specifies that a Subject is referred to by a given Source.</rdfs:comment>
  </owl:ObjectProperty>
  <owl:ObjectProperty rdf:about="http://discovery-project.eu/ontologies/scholar/0.1/defines">
    <rdfs:domain rdf:resource="http://discovery-project.eu/ontologies/scholar/0.1/Source"/>
    <owl:inverseOf>
      <owl:ObjectProperty rdf:about="http://discovery-project.eu/ontologies/scholar/0.1/isDefinedBy"/>
    </owl:inverseOf>
    <rdfs:comment xml:lang="en">This relation specifies that a Source gives a definition of a Subject.</rdfs:comment>
    <rdfs:range rdf:resource="http://discovery-project.eu/ontologies/scholar/0.1/Subject"/>
    <rdfs:subPropertyOf>
      <owl:ObjectProperty rdf:about="http://discovery-project.eu/ontologies/scholar/0.1/hasSubject"/>
    </rdfs:subPropertyOf>
    <rdfs:label xml:lang="en">defines</rdfs:label>
  </owl:ObjectProperty>
  <owl:ObjectProperty rdf:about="http://discovery-project.eu/ontologies/scholar/0.1/isExplainedIn">
    <owl:inverseOf>
      <owl:ObjectProperty rdf:about="http://discovery-project.eu/ontologies/scholar/0.1/explains"/>
    </owl:inverseOf>
    <rdfs:subPropertyOf rdf:resource="http://discovery-project.eu/ontologies/scholar/0.1/isSubjectOf"/>
    <rdfs:comment xml:lang="en">This relation is the inverse of the 'explains' relation. It specifies that a Subject is explaind by a given Source.</rdfs:comment>
    <rdfs:label xml:lang="en">is explained in</rdfs:label>
    <rdfs:domain rdf:resource="http://discovery-project.eu/ontologies/scholar/0.1/Subject"/>
  </owl:ObjectProperty>
  <owl:ObjectProperty rdf:about="http://discovery-project.eu/ontologies/scholar/0.1/isRelatedTo">
    <rdfs:comment xml:lang="en">This relation expresses a generic relation among a Source and and other Source.</rdfs:comment>
    <rdfs:domain rdf:resource="http://discovery-project.eu/ontologies/scholar/0.1/Source"/>
    <rdfs:label xml:lang="en">is related to</rdfs:label>
    <rdfs:range rdf:resource="http://discovery-project.eu/ontologies/scholar/0.1/Source"/>
  </owl:ObjectProperty>
  <owl:ObjectProperty rdf:about="http://discovery-project.eu/ontologies/scholar/0.1/hasSimilarContent">
    <rdfs:range rdf:resource="http://discovery-project.eu/ontologies/scholar/0.1/Source"/>
    <rdfs:comment xml:lang="en">This relation specifies that a Source has a similar content that an otehr Source have. For example the two Sources can express a similar view point on some topic or one can be a revision of the other.</rdfs:comment>
    <rdfs:label xml:lang="en">has similar content</rdfs:label>
    <rdfs:subPropertyOf rdf:resource="http://discovery-project.eu/ontologies/scholar/0.1/isRelatedTo"/>
    <rdfs:domain rdf:resource="http://discovery-project.eu/ontologies/scholar/0.1/Source"/>
  </owl:ObjectProperty>
  <owl:ObjectProperty rdf:about="http://discovery-project.eu/ontologies/scholar/0.1/isDefinedBy">
    <rdfs:subPropertyOf rdf:resource="http://discovery-project.eu/ontologies/scholar/0.1/isSubjectOf"/>
    <owl:inverseOf rdf:resource="http://discovery-project.eu/ontologies/scholar/0.1/defines"/>
    <rdfs:range rdf:resource="http://discovery-project.eu/ontologies/scholar/0.1/Source"/>
    <rdfs:label xml:lang="en">is defined by</rdfs:label>
    <rdfs:comment xml:lang="en">This relation is the inverse of the 'defines' relation. It specifies that a Subject is defined by a given Source.</rdfs:comment>
    <rdfs:domain rdf:resource="http://discovery-project.eu/ontologies/scholar/0.1/Subject"/>
  </owl:ObjectProperty>
  <owl:ObjectProperty rdf:about="http://discovery-project.eu/ontologies/scholar/0.1/hasAuthor">
    <rdfs:domain rdf:resource="http://discovery-project.eu/ontologies/scholar/0.1/Source"/>
    <rdfs:range rdf:resource="http://discovery-project.eu/ontologies/scholar/0.1/Person"/>
    <rdfs:comment xml:lang="en">The author of a Source is the human being (Person) who produced it.</rdfs:comment>
    <owl:inverseOf rdf:resource="http://discovery-project.eu/ontologies/scholar/0.1/isAuthorOf"/>
    <rdfs:label xml:lang="en">has author</rdfs:label>
  </owl:ObjectProperty>
  <owl:ObjectProperty rdf:about="http://discovery-project.eu/ontologies/scholar/0.1/quotes">
    <rdfs:comment xml:lang="en">This relation specifies that a Source quotes an other Source.</rdfs:comment>
    <rdfs:range rdf:resource="http://discovery-project.eu/ontologies/scholar/0.1/Source"/>
    <rdfs:domain rdf:resource="http://discovery-project.eu/ontologies/scholar/0.1/Source"/>
    <rdfs:subPropertyOf rdf:resource="http://discovery-project.eu/ontologies/scholar/0.1/isRelatedTo"/>
    <rdfs:label xml:lang="en">quotes</rdfs:label>
  </owl:ObjectProperty>
  <owl:ObjectProperty rdf:about="http://discovery-project.eu/ontologies/scholar/0.1/hasSubject">
    <rdfs:label xml:lang="en">has subject</rdfs:label>
    <owl:inverseOf rdf:resource="http://discovery-project.eu/ontologies/scholar/0.1/isSubjectOf"/>
    <rdfs:domain rdf:resource="http://discovery-project.eu/ontologies/scholar/0.1/Source"/>
    <rdfs:range rdf:resource="http://discovery-project.eu/ontologies/scholar/0.1/Subject"/>
    <rdfs:comment xml:lang="en">This relation specifies that a Source mentions or talks about a Subject. It is a generic relation as it does not specify the exact connection the Source as with the Subject.</rdfs:comment>
  </owl:ObjectProperty>
  <owl:ObjectProperty rdf:about="http://discovery-project.eu/ontologies/scholar/0.1/hasPart">
    <rdfs:range rdf:resource="http://discovery-project.eu/ontologies/scholar/0.1/Source"/>
    <rdfs:label xml:lang="en">has part</rdfs:label>
    <owl:inverseOf rdf:resource="http://discovery-project.eu/ontologies/scholar/0.1/isPartOf"/>
    <rdfs:domain rdf:resource="http://discovery-project.eu/ontologies/scholar/0.1/Source"/>
    <rdfs:comment xml:lang="en">This relation specifies that a Source is composed by an other Source. For example a page is a part of the entire book.</rdfs:comment>
  </owl:ObjectProperty>
  <owl:ObjectProperty rdf:about="http://discovery-project.eu/ontologies/scholar/0.1/explains">
    <rdfs:domain rdf:resource="http://discovery-project.eu/ontologies/scholar/0.1/Source"/>
    <rdfs:range rdf:resource="http://discovery-project.eu/ontologies/scholar/0.1/Subject"/>
    <owl:inverseOf rdf:resource="http://discovery-project.eu/ontologies/scholar/0.1/isExplainedIn"/>
    <rdfs:comment xml:lang="en">This relation specifies that a Source gives an explanation of a Subject.</rdfs:comment>
    <rdfs:subPropertyOf rdf:resource="http://discovery-project.eu/ontologies/scholar/0.1/hasSubject"/>
    <rdfs:label xml:lang="en">explains</rdfs:label>
  </owl:ObjectProperty>
  <owl:ObjectProperty rdf:about="http://discovery-project.eu/ontologies/scholar/0.1/isLocatedIn">
    <rdfs:comment xml:lang="en">This relation specifies the place where an entity is geografically located. For example a painting can be inside a building.</rdfs:comment>
    <rdfs:range rdf:resource="http://discovery-project.eu/ontologies/scholar/0.1/Place"/>
    <rdfs:label xml:lang="en">is located in</rdfs:label>
  </owl:ObjectProperty>
  <rdf:Description rdf:about="http://discovery-project.eu/ontologies/scholar/0.1/PhisicalObject">
    <rdfs:label rdf:datatype="http://www.w3.org/2001/XMLSchema#string"
    >Physical Object</rdfs:label>
  </rdf:Description>
</rdf:RDF>

<!-- Created with Protege (with OWL Plugin 3.4.4, Build 579)  http://protege.stanford.edu -->
